

Exercise 2

1. Jacobi-Matrix

$$f(u, v) = R \begin{pmatrix} \cos(u) \\ \sin(u) \\ 0 \end{pmatrix} + r \begin{pmatrix} \cos(u) \cos(v) \\ \sin(u) \cos(v) \\ \sin(v) \end{pmatrix}$$

$$\Leftrightarrow \begin{pmatrix} R \cdot \cos(u) + r \cos(u) \cos(v) \\ R \sin(u) + r \sin(u) \cos(v) \\ r \sin(v) \end{pmatrix} \begin{matrix} \rightarrow f_1 \\ \rightarrow f_2 \\ \rightarrow f_3 \end{matrix}$$

Jacobi-Matrix von $f(u, v)$:

$$\Rightarrow \begin{pmatrix} f'_{1u} & f'_{1v} \\ f'_{2u} & f'_{2v} \\ f'_{3u} & f'_{3v} \end{pmatrix} = \begin{pmatrix} -R \sin(u) - r \sin(u) \cos(v) & -r \cos(u) \sin(v) \\ R \cos(u) + r \cos(u) \cos(v) & -r \sin(u) \sin(v) \\ 0 & r \cos(v) \end{pmatrix}$$

2. First Fundamental Form

$$\underline{s} \begin{pmatrix} u \\ v \end{pmatrix} = \begin{pmatrix} R \cdot \cos(u) + r \cos(u) \cos(v) \\ R \sin(u) + r \sin(u) \cos(v) \\ r \sin(v) \end{pmatrix}$$

$$\underline{s}_u \begin{pmatrix} u \\ v \end{pmatrix} = \begin{pmatrix} -R \sin(u) - r \sin(u) \cos(v) \\ R \cos(u) + r \cos(u) \cos(v) \\ 0 \end{pmatrix} \quad \underline{s}_v \begin{pmatrix} u \\ v \end{pmatrix} = \begin{pmatrix} -r \cos(u) \sin(v) \\ -r \sin(u) \sin(v) \\ r \cos(v) \end{pmatrix}$$

$$\underline{I}_{\underline{s}} = \begin{pmatrix} E & F \\ F & G \end{pmatrix}$$

$$E = \underline{s}_u^2 = (-R \sin(u) - r \sin(u) \cos(v))^2 + (R \cos(u) + r \cos(u) \cos(v))^2 + 0$$

$$= \underbrace{(R^2 \sin(u)^2)} + \underbrace{2Rr \sin(u)^2 \cos(v)} + \underbrace{r^2 \sin(u)^2 \cos(v)^2} + \underbrace{R^2 \cos(u)^2} + \underbrace{2Rr \cos(u)^2 \cos(v)} + \underbrace{r^2 \cos(u)^2 \cos(v)^2}$$

$$= R^2 (\underbrace{\sin(u)^2 + \cos(u)^2}_{=1}) + 2Rr \cos(v) (\underbrace{\sin(u)^2 + \cos(u)^2}_{=1}) + r^2 \cos(v)^2 (\underbrace{\sin(u)^2 + \cos(u)^2}_{=1})$$

$$= R^2 + 2Rr \cos(v) + r^2 \cos(v)^2$$

$$= (R + r \cos(v))^2$$

$$G = \underline{s}_v^2 = r^2 \cos(u)^2 \sin(v)^2 + r^2 \sin(u)^2 \sin(v)^2 + r^2 \cos(v)^2$$

$$= r^2 \underbrace{\sin(v)^2} (\underbrace{\cos(u)^2 + \sin(u)^2}_{=1}) + r^2 \underbrace{\cos(v)^2}_{=1}$$

$$= r^2$$

$$\underline{s}_u \begin{pmatrix} u \\ v \end{pmatrix} = \begin{pmatrix} -R \sin(u) - r \sin(u) \cos(v) \\ R \cos(u) + r \cos(u) \cos(v) \\ 0 \end{pmatrix} \quad \underline{s}_v \begin{pmatrix} u \\ v \end{pmatrix} = \begin{pmatrix} -r \cos(u) \sin(v) \\ -r \sin(u) \sin(v) \\ r \cos(v) \end{pmatrix}$$

$$\tau = \langle \underline{s}_u, \underline{s}_v \rangle$$

$$= Rr \sin(u) \cos(u) \sin(v) + r^2 \sin(u) \cos(v) \cos(u) \sin(v) - Rr \cos(u) \sin(u) \sin(v) - r^2 \cos(u) \cos(v) \sin(u) \sin(v) + 0$$

$$= 0$$

$$I_{\frac{s}{r}} = \begin{pmatrix} E & F \\ F & G \end{pmatrix} = \begin{pmatrix} (R + r \cos(v))^2 & 0 \\ 0 & r^2 \end{pmatrix}$$

c) Surface Area

$$A = \int_{-\frac{\pi}{2}}^{\frac{\pi}{2}} \int_{-\pi}^{\pi} \sqrt{\det I_{\frac{s}{r}}} \, du \, dv$$

$$\Rightarrow \sqrt{\det I_{\frac{s}{r}}} : \begin{pmatrix} (R + r \cos(v))^2 & 0 \\ 0 & r^2 \end{pmatrix}$$

$$= \sqrt{r^2 \cdot (R + r \cos(v))^2}$$

$$= |r (R + r \cos(v))|$$

$$\Rightarrow A = \int_0^{2\pi} \int_0^{2\pi} |Rr + r^2 \cos(v)| \, du \, dv$$

$$= \int_0^{2\pi} \int_0^{2\pi} Rr \, du \, dv + \int_0^{2\pi} \int_0^{2\pi} r^2 \cos(v) \, du \, dv$$

$$= 2\pi Rr \int_0^{2\pi} dv + 2\pi r^2 \int_0^{2\pi} \cos(v) \, dv \quad \xrightarrow{\sin(2\pi) - \sin(0) = 0 + 0 = 0}$$

$$= 4\pi^2 Rr //$$